src/translation/HTLgen.v
@@ -16,6 +16,9 @@
  * along with this program.  If not, see <https://www.gnu.org/licenses/>.
  *)
 
+Require Import List.
+Import ListNotations.
+
 From compcert Require Import Maps.
 From compcert Require Errors Globalenvs Integers.
 From compcert Require Import AST RTL.
@@ -33,7 +36,7 @@ Record state: Type := mkstate {
   st_freshstate: node;
   st_scldecls: AssocMap.t (option io * scl_decl);
   st_arrdecls: AssocMap.t (option io * arr_decl);
-  (* TODO Add module declarations *)
+  st_insts: AssocMap.t instantiation;
   st_datapath: datapath;
   st_controllogic: controllogic;
 }.
@@ -44,6 +47,7 @@ Definition init_state (st : reg) : state :=
           1%positive
           (AssocMap.empty (option io * scl_decl))
           (AssocMap.empty (option io * arr_decl))
+          (AssocMap.empty instantiation)
           (AssocMap.empty stmnt)
           (AssocMap.empty stmnt).
 
@@ -60,6 +64,8 @@ Module HTLState <: State.
         (forall n,
             s1.(st_datapath)!n = None \/ s2.(st_datapath)!n = s1.(st_datapath)!n) ->
         (forall n,
+            s1.(st_insts)!n = None \/ s2.(st_insts)!n = s1.(st_insts)!n) ->
+        (forall n,
             s1.(st_controllogic)!n = None
             \/ s2.(st_controllogic)!n = s1.(st_controllogic)!n) ->
         st_incr s1 s2.
@@ -74,8 +80,9 @@ Module HTLState <: State.
     forall s1 s2 s3, st_prop s1 s2 -> st_prop s2 s3 -> st_prop s1 s3.
   Proof.
     intros. inv H. inv H0. apply state_incr_intro; eauto using Ple_trans; intros; try congruence.
-    - destruct H4 with n; destruct H8 with n; intuition congruence.
-    - destruct H5 with n; destruct H9 with n; intuition congruence.
+    - destruct H4 with n; destruct H9 with n; intuition congruence.
+    - destruct H5 with n; destruct H10 with n; intuition congruence.
+    - destruct H6 with n; destruct H11 with n; intuition congruence.
   Qed.
 
 End HTLState.
@@ -117,6 +124,7 @@ Lemma add_instr_state_incr :
        (st_freshstate s)
        s.(st_scldecls)
        s.(st_arrdecls)
+       s.(st_insts)
        (AssocMap.set n st s.(st_datapath))
        (AssocMap.set n (state_goto s.(st_st) n') s.(st_controllogic))).
 Proof.
@@ -134,6 +142,7 @@ Lemma declare_reg_state_incr :
        s.(st_freshstate)
        (AssocMap.set r (i, VScalar sz) s.(st_scldecls))
        s.(st_arrdecls)
+       s.(st_insts)
        s.(st_datapath)
        s.(st_controllogic)).
 Proof. auto with htlh. Qed.
@@ -145,6 +154,7 @@ Definition declare_reg (i : option io) (r : reg) (sz : nat) : mon unit :=
                 s.(st_freshstate)
                 (AssocMap.set r (i, VScalar sz) s.(st_scldecls))
                 s.(st_arrdecls)
+                s.(st_insts)
                 s.(st_datapath)
                 s.(st_controllogic))
               (declare_reg_state_incr i s r sz).
@@ -159,6 +169,7 @@ Definition add_instr (n : node) (n' : node) (st : stmnt) : mon unit :=
                (st_freshstate s)
                s.(st_scldecls)
                s.(st_arrdecls)
+               s.(st_insts)
                (AssocMap.set n st s.(st_datapath))
                (AssocMap.set n (state_goto s.(st_st) n') s.(st_controllogic)))
          (add_instr_state_incr s n n' st STM TRANS)
@@ -176,6 +187,7 @@ Lemma add_instr_skip_state_incr :
        (st_freshstate s)
        s.(st_scldecls)
        s.(st_arrdecls)
+       s.(st_insts)
        (AssocMap.set n st s.(st_datapath))
        (AssocMap.set n Vskip s.(st_controllogic))).
 Proof.
@@ -194,6 +206,7 @@ Definition add_instr_skip (n : node) (st : stmnt) : mon unit :=
                (st_freshstate s)
                s.(st_scldecls)
                s.(st_arrdecls)
+               s.(st_insts)
                (AssocMap.set n st s.(st_datapath))
                (AssocMap.set n Vskip s.(st_controllogic)))
          (add_instr_skip_state_incr s n st STM TRANS)
@@ -211,6 +224,7 @@ Lemma add_node_skip_state_incr :
        (st_freshstate s)
        s.(st_scldecls)
        s.(st_arrdecls)
+       s.(st_insts)
        (AssocMap.set n Vskip s.(st_datapath))
        (AssocMap.set n st s.(st_controllogic))).
 Proof.
@@ -229,11 +243,51 @@ Definition add_node_skip (n : node) (st : stmnt) : mon unit :=
                (st_freshstate s)
                s.(st_scldecls)
                s.(st_arrdecls)
+               s.(st_insts)
                (AssocMap.set n Vskip s.(st_datapath))
                (AssocMap.set n st s.(st_controllogic)))
          (add_node_skip_state_incr s n st STM TRANS)
     | _, _ => Error (Errors.msg "HTL.add_instr")
     end.
+
+Fixpoint assocmap_nextavailable {A: Type} (m: AssocMap.t A) : positive :=
+  match m with
+  | AssocMap.Leaf => 1
+  | AssocMap.Node _ _ r => (assocmap_nextavailable r)~1
+  end.
+
+Theorem assocmap_nextavailable_correct : forall (A: Type) m, m!(@assocmap_nextavailable A m) = None.
+Proof. induction m; tauto. Qed.
+
+Lemma add_instance_state_incr :
+  forall s inst,
+    st_incr s
+      (mkstate
+        s.(st_st)
+        s.(st_freshreg)
+        s.(st_freshstate)
+        s.(st_scldecls)
+        s.(st_arrdecls)
+        (AssocMap.set (assocmap_nextavailable s.(st_insts)) inst s.(st_insts))
+        s.(st_datapath)
+        s.(st_controllogic)).
+Proof.
+Admitted.
+
+Definition add_instance (mod_name: ident) (args: list reg) (rst: reg) (finished: reg) (dst: reg) : mon unit :=
+  fun s =>
+        let instname := assocmap_nextavailable s.(st_insts) in
+        let inst := Vinstantiation mod_name instname ([rst] ++ args ++ [finished; dst]) in
+        OK tt (mkstate
+              s.(st_st)
+              s.(st_freshreg)
+              s.(st_freshstate)
+              s.(st_scldecls)
+              s.(st_arrdecls)
+              (AssocMap.set instname inst s.(st_insts))
+              s.(st_datapath)
+              s.(st_controllogic))
+       (add_instance_state_incr s inst).
 
 Definition nonblock (dst : reg) (e : expr) := Vnonblock (Vvar dst) e.
 Definition block (dst : reg) (e : expr) := Vblock (Vvar dst) e.
@@ -387,6 +441,7 @@ Lemma add_branch_instr_state_incr:
                 (st_freshstate s)
                 s.(st_scldecls)
                 s.(st_arrdecls)
+                s.(st_insts)
                 (AssocMap.set n Vskip (st_datapath s))
                 (AssocMap.set n (state_cond s.(st_st) e n1 n2) (st_controllogic s))).
 Proof.
@@ -405,6 +460,7 @@ Definition add_branch_instr (e: expr) (n n1 n2: node) : mon unit :=
                 (st_freshstate s)
                 s.(st_scldecls)
                 s.(st_arrdecls)
+                s.(st_insts)
                 (AssocMap.set n Vskip (st_datapath s))
                 (AssocMap.set n (state_cond s.(st_st) e n1 n2) (st_controllogic s)))
          (add_branch_instr_state_incr s e n n1 n2 NSTM NTRANS)
@@ -445,6 +501,32 @@ Definition tbl_to_case_expr (st : reg) (ns : list node) : list (expr * stmnt) :=
                   end)
            (enumerate 0 ns).
 
+Lemma create_reg_state_incr:
+  forall s sz i,
+    st_incr s (mkstate
+         s.(st_st)
+         (Pos.succ (st_freshreg s))
+         (st_freshstate s)
+         (AssocMap.set s.(st_freshreg) (i, VScalar sz) s.(st_scldecls))
+         s.(st_arrdecls)
+         s.(st_insts)
+         (st_datapath s)
+         (st_controllogic s)).
+Proof. constructor; simpl; auto with htlh. Qed.
+
+Definition create_reg (i : option io) (sz : nat) : mon reg :=
+  fun s => let r := s.(st_freshreg) in
+           OK r (mkstate
+                   s.(st_st)
+                   (Pos.succ r)
+                   (st_freshstate s)
+                   (AssocMap.set s.(st_freshreg) (i, VScalar sz) s.(st_scldecls))
+                   (st_arrdecls s)
+                   (st_insts s)
+                   (st_datapath s)
+                   (st_controllogic s))
+              (create_reg_state_incr s sz i).
+
 Definition transf_instr (fin rtrn stack: reg) (ni: node * instruction) : mon unit :=
   match ni with
     (n, i) =>
@@ -473,9 +555,9 @@ Definition transf_instr (fin rtrn stack: reg) (ni: node * instruction) : mon uni
     | Icall sig (inl fn) args dst n' => error (Errors.msg "Indirect calls are not implemented.")
     | Icall sig (inr fn) args dst n' =>
       if Z.leb (Z.pos n') Integers.Int.max_unsigned then
-      (* TODO Find calling convention for VeriCert-generated modules *)
-      (* TODO Generate an ident for instantiated modules (fresh name supply?) *)
-        add_instr n n' (Vinstantiate fn 1%positive (dst :: args))
+        do rst <- create_reg None 1;
+        do finished <- create_reg None 1;
+        add_instance fn args rst finished dst
       else error (Errors.msg "State is larger than 2^32.")
     | Itailcall _ _ _ => error (Errors.msg "Tailcalls are not implemented.")
     | Ibuiltin _ _ _ _ => error (Errors.msg "Builtin functions not implemented.")
@@ -498,30 +580,6 @@ Definition transf_instr (fin rtrn stack: reg) (ni: node * instruction) : mon uni
     end
   end.
 
-Lemma create_reg_state_incr:
-  forall s sz i,
-    st_incr s (mkstate
-         s.(st_st)
-         (Pos.succ (st_freshreg s))
-         (st_freshstate s)
-         (AssocMap.set s.(st_freshreg) (i, VScalar sz) s.(st_scldecls))
-         s.(st_arrdecls)
-         (st_datapath s)
-         (st_controllogic s)).
-Proof. constructor; simpl; auto with htlh. Qed.
-
-Definition create_reg (i : option io) (sz : nat) : mon reg :=
-  fun s => let r := s.(st_freshreg) in
-           OK r (mkstate
-                   s.(st_st)
-                   (Pos.succ r)
-                   (st_freshstate s)
-                   (AssocMap.set s.(st_freshreg) (i, VScalar sz) s.(st_scldecls))
-                   (st_arrdecls s)
-                   (st_datapath s)
-                   (st_controllogic s))
-              (create_reg_state_incr s sz i).
-
 Lemma create_arr_state_incr:
   forall s sz ln i,
     st_incr s (mkstate
@@ -530,6 +588,7 @@ Lemma create_arr_state_incr:
          (st_freshstate s)
          s.(st_scldecls)
          (AssocMap.set s.(st_freshreg) (i, VArray sz ln) s.(st_arrdecls))
+         (st_insts s)
          (st_datapath s)
          (st_controllogic s)).
 Proof. constructor; simpl; auto with htlh. Qed.
@@ -542,6 +601,7 @@ Definition create_arr (i : option io) (sz : nat) (ln : nat) : mon (reg * nat) :=
                    (st_freshstate s)
                    s.(st_scldecls)
                    (AssocMap.set s.(st_freshreg) (i, VArray sz ln) s.(st_arrdecls))
+                   (st_insts s)
                    (st_datapath s)
                    (st_controllogic s))
               (create_arr_state_incr s sz ln i).
@@ -605,6 +665,7 @@ Definition transf_module (f: function) : mon module :=
            start
            rst
            clk
+           current_state.(st_insts)
            current_state.(st_scldecls)
            current_state.(st_arrdecls)
            (conj (max_pc_wf _ LECTRL) (max_pc_wf _ LEDATA)))
@@ -619,6 +680,7 @@ Definition max_state (f: function) : state :=
           (Pos.succ (max_pc_function f))
           (AssocMap.set st (None, VScalar 32) (st_scldecls (init_state st)))
           (st_arrdecls (init_state st))
+          (st_insts (init_state st))
           (st_datapath (init_state st))
           (st_controllogic (init_state st)).
 
